\documentclass[]{article}

%opening
\title{Assignment 3}
\author{Colin Gagich}
\date{\today}

\renewcommand\thesection{\alph{section}$)$ }

\begin{document}

\maketitle

\section{}

Differentiating $y = C e^{3t} + e^{-t}$ we get:

\begin{center}
$\frac{dy}{dt} y = 3 C e^{3t} - e^{-t}$
\end{center}

Then, we re-arrange our first equation:

\begin{center}
$C e^{3t} = y - e^{-t}$
\end{center}

And substitute it into the second equation:

\begin{center}
$y' = 3 (y - e^{-t}) - e^{-t}$ \\
$y' = 3 y - 4 e^{-t}$\\
\end{center}

\noindent Therefore $y = C e^{3t} + e^{-t}$ is indeed a general analytic solution to the equation $y' = 3 y - 4 e^{-t}$.

\section{}

Substituting the values $y = 1$ and $t = 0$ into $y = C e^{3t} + e^{-t}$

\begin{center}
$1 = C e^{0} + e^{0}$ \\
$1 = C + 1$ \\
\end{center}

\noindent Therefore $C = 0$, substituting this back in the proposed solution we find the analytic solution is indeed $y = e^{-t}$

\newpage
\section{}

Using a computer program written in C$^{\#}$ the following values were obtained:

\begin{center}
$y(0) = 1$\\
$y(1) = 0.367741025173408$\\
$y(2) = 0.132504642015483$\\
$y(3) = -0.00707763902447456$\\
$y(4) = -1.1236691550673$\\
$y(5) = -22.9270219157003$\\
$y(6) = -460.561696136583$\\
$y(7) = -9249.21770901647$\\
$y(8) = -185746.199126798$\\
$y(9) = -3730223.27913773$\\
$y(10) = -74911711.536581$\\
\end{center}

\end{document}
